compiler/backend/proofs/word_to_stackProofScript.sml
@@ -5490,15 +5490,15 @@ val comp_correct = Q.store_thm("comp_correct",
        >> metis_tac[IS_PREFIX_TRANS,comp_IMP_isPREFIX,evaluate_consts])>>
     strip_tac>>qexists_tac`ck`>>rfs[])
   THEN1 (* LocValue *) (
-    qexists_tac`0` \\ simp[]
-    \\ fs[wordSemTheory.evaluate_def]
-    \\ rw[comp_def,stackSemTheory.evaluate_def]
+    fs[comp_def,wordSemTheory.evaluate_def]
     \\ fs[convs_def,reg_allocTheory.is_phy_var_def,GSYM EVEN_MOD2,EVEN_EXISTS]
-    \\ simp[TWOxDIV2]
-    \\ match_mp_tac state_rel_set_var
-    \\ fs[word_allocTheory.max_var_def,GSYM LEFT_ADD_DISTRIB]
-    \\ rveq \\ fs[]
-    \\ cheat (* syntactic conventions not good enough? *))
+    \\ rw[]
+    \\ qexists_tac`0` \\ simp[]
+    \\ CONV_TAC SWAP_EXISTS_CONV
+    \\ qexists_tac`NONE` \\ simp[]
+    \\ match_mp_tac wRegWrite1_thm1
+    \\ simp[stackSemTheory.evaluate_def]
+    \\ fs[word_allocTheory.max_var_def,GSYM LEFT_ADD_DISTRIB])
   THEN1 (* FFI *)
    (fs [EVAL ``post_alloc_conventions k (FFI ffi_index ptr len names)``]
     \\ rw [] \\ fs [] \\ rw []
